\newcommand{\E}{\mathrm{E}}
\newcommand{\Var}{\mathrm{Var}}
For a Poisson variable X,
\begin{align}
\pr{X=k} = \frac{\lambda^{k}e^{-\lambda}}{k!}
\end{align}
Since $\pr{X_1=2} = \pr{X_1=1}$,
\begin{align}
\frac{{\lambda_1}^{2}e^{-{\lambda_1}}}{2!} &= \frac{{\lambda_1}^{1}e^{-{\lambda_1}}}{1!} \\
\lambda_1 &= 2!/1! = 2
\end{align}
Similarly, as $\pr{X_2=2} = \pr{X_2=3}$,
\begin{align}
\frac{{\lambda_2}^{2}e^{-{\lambda_2}}}{2!} &= \frac{{\lambda_2}^{3}e^{-{\lambda_2}}}{3!} \\
\lambda_2 &= 3!/2! = 3
\end{align}
Also we know for a Poisson variable X, the following holds true:
\begin{align}
\E[X] &= \lambda \\
\Var[X] &= \lambda \label{2016/4eq1} \\
\Var[X] &= \E[X^2] - (\E[X])^2 \label{2016/4eq2} 
\end{align}
Now, for the variance of $(X_1 - 2X_2)$
\begin{align}
\Var[X_1 - 2X_2] &= \E[(X_1 - 2X_2)^2] - (\E[X_1 - 2X_2])^2 \nonumber \\
&= \E[X_1^2 + 4X_2^2 - 4X_1X_2] \nonumber \\
&- (\E[X_1] - 2\E[X_2])^2 \nonumber \\
&= \E[X_1^2] - (\E[X_1])^2 + 4\E[X_2^2] \nonumber \\
& -4(\E[X_2])^2) + 4\E[X_1X_2] \nonumber \\
& + 4\E[X_1]\E[X_2]
\end{align}
Since the variables are independent:
\begin{align}
\E[X_1X_2] = \E[X_1]\E[X_2]
\end{align}
Substituting equations \eqref{2016/4eq1} and \eqref{2016/4eq2}, we get:
\begin{align}
\Var[X_1 - 2X_2] &= \Var[X_1] + 4(\Var[X_2]) \nonumber \\
&- 4\E[X_1][X_2] + 4\E[X_1][X_2] \nonumber \\
&= \lambda_1 + 4\lambda_2 = 2 + 4(3) = 14
\end{align}
Hence option (a) 14 is correct.