
Let the abbreviations LE and LIE denote linearity of expectations and law of iterated expectations respectively.
\begin{align}
Var [Y] &= E[Y^2] -[E(Y)]^2\text{  (definition)  }\\
        &= E[E(Y^2 | X )] - (E[E(Y | X)])^2\text{  (LIE)  }
\end{align}
\begin{multline}
    =E[E(Y^2 | X )] - (E[E(Y | X)])^2\\-E([E(Y | X)]^2) + E([E(Y | X)]^2)
\end{multline}
\begin{multline}
        =E[E(Y^2 | X )] - E([E(Y | X)]^2) \\ + E([E(Y | X)]^2) - (E[E(Y | X)])^2\text{  (LE {\&} LIE)  }
\end{multline}
\begin{align}
        &= Var [E(Y | X)] + E[Var (Y | X)]\text{  (definition)  }
\end{align}
\bigskip
\rightline{Hence, proved.}